Boogie/Lambda Type Inference/Partial Evaluation Perf. Improvements (#94)
*Description of changes:*

*Lambda*

- Changed representation of a `KnownType` from being an `LTy` to a
structure that keeps track of the type name and arity. This restriction
(because `LTy` is more expressive) disallows the undesirable situation
where a user could define an `.ftvar` as a known type -- all known types
are always interpreted as `.tcons` now. This change also simplifies
_and_ optimizes the definition of the frequently-called function
`isInstanceOfKnownType` by removing the need for unification.

- Changed the representation of a `TypeAlias` to simplify the
implementation of `resolveAliases`. Add `TEnv.addTypeAlias` that
performs well-formedness checks before registering a known type alias in
the environment.

- Made many functions like `LExprT.fromLExprs`, `LMonoTys.subst`,
`LState.genVars`, `LState.knownVars`, etc. tail-recursive for
efficiency.

*Imperative*

- `EvalContext.preprocess` also takes the command as a parameter now to
allow the user to do command-specific preprocessing.

*Boogie*

- Disallow redefinition of type declarations/aliases.
  
- Rewrote `OldExpressions.substsOldExpr` to be efficient.
  
- Avoid unnecessary computation of free variables during PE.
  
- Avoid checking that `Env.genVar'` truly generates fresh variables,
instead relying on `Env.genSym` being correct.
  
- Make `Program.typeCheck`, `Statement.typeCheckAux`, `Statement.subst`,
etc. tail-recursive.
    

TODO: Proofs in *WF.lean broken. @atomb 

By submitting this pull request, I confirm that you can use, modify,
copy, and redistribute this contribution, under the terms of your
choice.

Strata/DL/Lambda/LExprTypeEnv.lean
@@ -23,16 +23,33 @@ open LExpr
 
 ---------------------------------------------------------------------
 
+/--
+A type alias is syntactic sugar for a type definition. E.g.,
+`∀α. FooAlias α := Foo α` is represented in `TypeAlias` as follows; note that
+`α` is common to both the alias and its definition.
+```
+{
+  name := "FooAlias"
+  typeArgs := ["α"]
+  type := LMonoTy.tcons "Foo" [.ftvar "α"]
+}
+```
+
+IMPORTANT: we expect the type definition to not be an alias itself, to avoid any
+cycles. See function `TEnv.addTypeAlias` for a canonical way of adding
+well-formed type aliases to the context.
+-/
 structure TypeAlias where
-  args : List TyIdentifier
-  lhs  : LMonoTy
-  rhs  : LMonoTy
-  deriving DecidableEq, Repr
+  name : String
+  typeArgs : List TyIdentifier
+  type : LMonoTy
+  deriving DecidableEq, Repr, Inhabited
+
+def TypeAlias.toAliasLTy (a : TypeAlias) : LTy :=
+  .forAll a.typeArgs (.tcons a.name (a.typeArgs.map (fun i => .ftvar i)))
 
 instance : ToFormat TypeAlias where
-  format a :=
-    let pfx := if a.args.isEmpty then f!"" else f!"∀{Std.Format.joinSep a.args " "}."
-    f!"{pfx}{a.lhs} := {a.rhs}"
+  format t := f!"{t.toAliasLTy} := {t.type}"
 
 variable {Identifier : Type} [DecidableEq Identifier] [ToFormat Identifier]
 
@@ -44,7 +61,7 @@ their type schemes. This is essentially a stack to account for variable scopes.
 
 The `aliases` field maps type synonyms to their corresponding type definitions.
 We expect these type definitions to not be aliases themselves, to avoid any
-cycles in the map.
+cycles in the map (see `TEnv.addTypeAlias`).
 -/
 structure TContext (Identifier : Type) where
   types   :  Maps Identifier LTy := []
@@ -64,14 +81,6 @@ def TContext.knownVars (ctx : (TContext Identifier)) : List Identifier :=
   where go types :=
   match types with
   | [] => [] | m :: rest => m.keys ++ go rest
-
-/--
-Get all non-global variables in `ctx`, i.e., those that are not in the oldest
-context.
--/
-def TContext.nonGlobalVars (ctx : (TContext Identifier)) : List Identifier :=
-  let nonglobals := ctx.types.dropOldest
-  TContext.knownVars.go nonglobals
 
 def TContext.types.knownTypeVars (types : Maps Identifier LTy) : List TyIdentifier :=
   match types with
@@ -115,21 +124,11 @@ def TContext.types.subst (types : Maps Identifier LTy) (S : Subst) :
     | (x, ty) :: mrest =>
       (x, LTy.subst S ty) :: go mrest
 
-def TContext.aliases.subst (aliases : List TypeAlias) (S : Subst) :
-  List TypeAlias :=
-  match aliases with
-  | [] => []
-  | { args, lhs, rhs} :: arest =>
-    let lhs := (LTy.forAll args lhs).subst S |>.toMonoTypeUnsafe
-    let rhs := (LTy.forAll args rhs).subst S |>.toMonoTypeUnsafe
-    {args, lhs, rhs} :: aliases.subst arest S
-
 /--
 Apply a substitution `S` to the context.
 -/
 def TContext.subst (T : TContext Identifier) (S : Subst) : TContext Identifier :=
-  { T with types := types.subst T.types S,
-           aliases := aliases.subst T.aliases S }
+  { T with types := types.subst T.types S }
 
 ---------------------------------------------------------------------
 
@@ -180,8 +179,31 @@ instance : ToFormat TState where
 
 ---------------------------------------------------------------------
 
-/-- Track registered types. -/
-abbrev KnownTypes := List LTy
+/-- Name and arity of a registered type. -/
+structure KnownType where
+  name : String
+  arity : Nat := 0
+  deriving Inhabited, Repr, DecidableEq
+
+def KnownType.toLTy (k : KnownType) : LTy :=
+  let bvars := (List.range k.arity).map (fun a => toString a)
+  let args := bvars.map (fun b => .ftvar b)
+  .forAll bvars (.tcons k.name args)
+
+def LTy.toKnownType! (lty : LTy) : KnownType :=
+  match lty with
+  | .forAll _ (.tcons name args) => { name, arity := args.length }
+  | .forAll [] (.bitvec _) => { name := "bitvec", arity := 1 }
+  | _ => panic! s!"Unsupported known type: {lty}"
+
+instance : ToFormat KnownType where
+  format k := f!"{k.toLTy}"
+
+/-- Registered types. -/
+abbrev KnownTypes := List KnownType
+
+def KnownTypes.keywords (ks : KnownTypes) : List String :=
+  ks.map (fun k => k.name)
 
 /--
 A type environment `TEnv` contains a stack of contexts `TContext` to track `LExpr`
@@ -196,15 +218,20 @@ structure TEnv (Identifier : Type) where
   functions : @Factory Identifier
   knownTypes : KnownTypes
 
+def KnownTypes.default : KnownTypes :=
+  open LTy.Syntax in
+  [t[∀a b. %a → %b],
+   t[bool],
+   t[int],
+   t[string]].map (fun k => k.toKnownType!)
+
 def TEnv.default : TEnv Identifier :=
   open LTy.Syntax in
   { context := {},
     state := TState.init,
     functions := #[],
-    knownTypes := [t[∀a b. %a → %b],
-                   t[bool],
-                   t[int],
-                   t[string]] }
+    knownTypes := KnownTypes.default
+  }
 
 instance : ToFormat (TEnv Identifier) where
   format s := f!"context:{Format.line}{s.context}\
@@ -213,8 +240,8 @@ instance : ToFormat (TEnv Identifier) where
                  {Format.line}\
                  known types:{Format.line}{s.knownTypes}"
 
-def TEnv.addKnownType (T : TEnv Identifier) (lty : LTy) : TEnv Identifier :=
-  { T with knownTypes := lty :: T.knownTypes }
+def TEnv.addKnownType (T : TEnv Identifier) (k : KnownType) : TEnv Identifier :=
+  { T with knownTypes := k :: T.knownTypes }
 
 def TEnv.addFactoryFunction (T : TEnv Identifier) (fn : LFunc Identifier) : TEnv Identifier :=
   { T with functions := T.functions.push fn }
@@ -226,7 +253,7 @@ def TEnv.addFactoryFunctions (T : TEnv Identifier) (fact : @Factory Identifier) 
 Replace the global substitution in `T.state.subst` with `S`.
 -/
 def TEnv.updateSubst (T : (TEnv Identifier)) (S : SubstInfo) : (TEnv Identifier) :=
-  { T with state := { T.state with substInfo := S }}
+  { T with state.substInfo := S }
 
 def TEnv.pushEmptyContext (T : (TEnv Identifier)) : (TEnv Identifier) :=
   let ctx := T.context
@@ -355,8 +382,8 @@ def LMonoTys.instantiate (ids : List TyIdentifier) (mtys : LMonoTys) (T : (TEnv 
 omit [DecidableEq Identifier] in
 theorem LMonoTys.instantiate_length :
   (LMonoTys.instantiate (Identifier:=Identifier) ids mty T).fst.length == mty.length := by
-  simp [instantiate]
-  induction mty <;> simp_all [subst]
+  simp [instantiate, LMonoTys.subst_eq_substLogic]
+  induction mty <;> simp_all [substLogic]
 
 /--
 Instantiate the scheme `ty` by filling in fresh type variables for all
@@ -374,88 +401,95 @@ def LTy.instantiate (ty : LTy) (T : (TEnv Identifier)) : LMonoTy × (TEnv Identi
     let S := List.zip xs (List.map (fun tv => (.ftvar tv)) freshtvs)
     (LMonoTy.subst S lty', T)
 
+instance : Inhabited (Option LMonoTy × TEnv Identifier) where
+  default := (none, TEnv.default)
+
 /--
-Return the definition of `ty` if it is a type alias registered in the typing
-environment `T`.
+Return the instantiated definition of `ty` if it is a type alias registered in
+the typing environment `T`. This function does not descend into the subtrees of
+`mty`.
 -/
-def LTy.aliasDef? (mty : LMonoTy) (T : (TEnv Identifier)) : (Option LMonoTy × (TEnv Identifier)) :=
+def LMonoTy.aliasDef? (mty : LMonoTy) (T : (TEnv Identifier)) : (Option LMonoTy × TEnv Identifier) :=
   match mty with
   | .ftvar _ =>
     -- We can't have a free variable be the LHS of an alias definition because
     -- then it will unify with every type.
     (none, T)
-  | _ => go mty T.context.aliases T
-  where go (mty : LMonoTy) (aliases : List TypeAlias) (T : (TEnv Identifier)) :=
-  match aliases with
-  | [] => (none, T)
-  | { args, lhs, rhs } :: arest =>
-    let (mtys, T) := LMonoTys.instantiate args [lhs, rhs] T
-    match mtys with
-    | [lhsty, rhsty] =>
-      match Constraints.unify [(mty, lhsty)] T.state.substInfo with
-      | .error _ => go mty arest T
-      | .ok S => (rhsty.subst S.subst, T)
-    | _ =>
-      -- panic s!"[LTy.aliasBaseDef?] Implementation error!"
-      -- (FIXME) Prove that the following is unreachable.
-      (none, T)
+  | .bitvec _ =>
+    -- A bitvector cannot be a type alias.
+    (none, T)
+  | .tcons name args =>
+    match T.context.aliases.find? (fun a => a.name == name && a.typeArgs.length == args.length) with
+    | none => (none, T)
+    | some alias =>
+      let (lst, T) := LMonoTys.instantiate alias.typeArgs [(.tcons name (alias.typeArgs.map (fun a => .ftvar a))), alias.type] T
+      -- (FIXME): Use `LMonoTys.instantiate_length` to remove the `!` below.
+      let alias_inst := lst[0]!
+      let alias_def := lst[1]!
+      match Constraints.unify [(mty, alias_inst)] T.state.substInfo with
+      | .error e =>
+        panic! s!"[LMonoTy.aliasDef?] {e}"
+      | .ok S => (alias_def.subst S.subst, T)
 
 /-- info: none -/
 #guard_msgs in
 open LTy.Syntax in
-#eval LTy.aliasDef? mty[%__ty0] { @TEnv.default String with
-              context := { aliases := [{ args := ["x", "y"],
-                                          lhs := mty[myInt %x %y],
-                                          rhs := mty[int] }] }}
+#eval LMonoTy.aliasDef? mty[%__ty0] { @TEnv.default String with
+              context := { aliases := [{ typeArgs := ["x", "y"],
+                                         name := "myInt",
+                                         type := mty[int] }] }}
       |>.fst |>.format
-
 
 /-- info: some int -/
 #guard_msgs in
 open LTy.Syntax in
-#eval LTy.aliasDef? mty[myInt] { @TEnv.default String with
-          context := { aliases := [{ args := [],
-                                      lhs := mty[myInt],
-                                      rhs := mty[int]}]} }
+#eval LMonoTy.aliasDef? mty[myInt] { @TEnv.default String with
+          context := { aliases := [{ typeArgs := [],
+                                     name := "myInt",
+                                     type := mty[int]}]} }
       |>.fst |>.format
 
 /-- info: some bool -/
 #guard_msgs in
 open LTy.Syntax in
-#eval LTy.aliasDef?
+#eval LMonoTy.aliasDef?
         mty[FooAlias %p %q]
         { @TEnv.default String with
-          context := { aliases := [{ args := ["x", "y"],
-                                      lhs := mty[FooAlias %x %y],
-                                      rhs := mty[bool]}]} }
+          context := { aliases := [{ typeArgs := ["x", "y"],
+                                     name := "FooAlias",
+                                     type := mty[bool]}]} }
       |>.fst |>.format
 
 /-- info: none -/
 #guard_msgs in
 open LTy.Syntax in
-#eval LTy.aliasDef? mty[myInt]
+#eval LMonoTy.aliasDef? mty[myInt]
                     { @TEnv.default String with context := { aliases := [{
-                        args := ["a"],
-                         lhs := mty[myInt %a],
-                         rhs := mty[int]}] } }
+                         typeArgs := ["a"],
+                         name := "myInt",
+                         type := mty[int]}] } }
       |>.fst |>.format
 
 /-- info: some (myTy int) -/
 #guard_msgs in
 open LTy.Syntax in
-#eval LTy.aliasDef? mty[myInt int bool]
+#eval LMonoTy.aliasDef? mty[myInt int bool]
                     { @TEnv.default String with
                     context := {
                       aliases := [{
-                        args := ["a", "b"],
-                        lhs := mty[myInt %a %b],
-                        rhs := mty[myTy %a]}] },
-                      knownTypes := [t[∀a. myTy %a], t[int]] }
+                        typeArgs := ["a", "b"],
+                        name := "myInt",
+                        type := mty[myTy %a]}] },
+                      knownTypes := [{ name := "myTy", arity := 1 },
+                                     { name := "int", arity := 0 }] }
       |>.fst |>.format
 
 mutual
-def LMonoTy.aliasInst (mty : LMonoTy) (T : TEnv Identifier) : (Option LMonoTy × TEnv Identifier) :=
-  let (maybe_mty, T) := LTy.aliasDef? mty T
+/--
+De-alias `mty`, including at the subtrees.
+-/
+def LMonoTy.resolveAliases (mty : LMonoTy) (T : TEnv Identifier) : (Option LMonoTy × TEnv Identifier) :=
+  let (maybe_mty, T) := LMonoTy.aliasDef? mty T
   match maybe_mty with
   | some mty => (some mty, T)
   | none =>
@@ -463,61 +497,77 @@ def LMonoTy.aliasInst (mty : LMonoTy) (T : TEnv Identifier) : (Option LMonoTy ×
     | .ftvar _ => (some mty, T)
     | .bitvec _ => (some mty, T)
     | .tcons name mtys =>
-      let (maybe_mtys, T) := LMonoTys.aliasInst mtys T.context.aliases T
+      let (maybe_mtys, T) := LMonoTys.resolveAliases mtys T.context.aliases T
       match maybe_mtys with
       | none => (none, T)
       | some mtys' => (some (.tcons name mtys'), T)
 
-def LMonoTys.aliasInst (mtys : LMonoTys) (aliases : List TypeAlias) (T : (TEnv Identifier)) :
+/--
+De-alias `mtys`, including at the subtrees.
+-/
+def LMonoTys.resolveAliases (mtys : LMonoTys) (aliases : List TypeAlias) (T : (TEnv Identifier)) :
     (Option LMonoTys × (TEnv Identifier)) :=
     match mtys with
     | [] => (some [], T)
     | mty :: mrest =>
-      let (mty', T) := LMonoTy.aliasInst mty T
-      let (mrest', T) := LMonoTys.aliasInst mrest aliases T
+      let (mty', T) := LMonoTy.resolveAliases mty T
+      let (mrest', T) := LMonoTys.resolveAliases mrest aliases T
       if h : mty'.isSome && mrest'.isSome then
         ((mty'.get (by simp_all) :: mrest'.get (by simp_all)), T)
       else
         (none, T)
 end
 
-def LTy.aliasInst (ty : LTy) (T : (TEnv Identifier)) : (Option LMonoTy × (TEnv Identifier)) :=
+/--
+Instantiate and de-alias `ty`, including at the subtrees.
+-/
+def LTy.resolveAliases (ty : LTy) (T : (TEnv Identifier)) : (Option LMonoTy × (TEnv Identifier)) :=
   let (mty, T) := ty.instantiate T
-  LMonoTy.aliasInst mty T
-
+  LMonoTy.resolveAliases mty T
 
 /-- info: some (arrow bool $__ty0) -/
 #guard_msgs in
 open LTy.Syntax in
-#eval LTy.aliasInst
+#eval LTy.resolveAliases
         t[∀x. (FooAlias %x %x) → %x]
         { @TEnv.default String with context := { aliases := [{
-                                        args := ["x", "y"],
-                                        lhs := mty[FooAlias %x %y],
-                                        rhs := mty[bool]}]} }
+                                        typeArgs := ["x", "y"],
+                                        name := "FooAlias",
+                                        type := mty[bool]}]} }
       |>.fst |>.format
 
+mutual
 /--
-Is `ty` an instance of a previously registered type?
+Is `ty` an instance of a known type in `ks`? We expect `ty` to be
+de-aliased.
 -/
-def isInstanceOfKnownType (ty : LMonoTy) (T : (TEnv Identifier)) : Bool :=
-  let tys := ty.getTyConstructors
-  tys.all (fun ty => go ty T.knownTypes T.state.substInfo T)
-  where go ty (knownTys : KnownTypes) S T : Bool :=
-    match knownTys with
-    | [] => false
-    | k :: krest =>
-      let (km, T) := LTy.instantiate k T
-      match Constraints.unify [(km, ty)] S with
-      | .error _ => go ty krest S T
-      | .ok _ => true
+def LMonoTy.knownInstance (ty : LMonoTy) (ks : KnownTypes) : Bool :=
+  match ty with
+  | .ftvar _ | .bitvec _ => true
+  | .tcons name args =>
+    (ks.contains { name := name, arity := args.length }) &&
+    LMonoTys.knownInstances args ks
+
+/--
+Are `tys` instances of some known type in `ks`? We expect all types in
+`tys` to be de-aliased.
+-/
+def LMonoTys.knownInstances (tys : LMonoTys) (ks : KnownTypes) : Bool :=
+  match tys with
+  | [] => true
+  | ty :: trest =>
+    if LMonoTy.knownInstance ty ks then LMonoTys.knownInstances trest ks else false
+end
+
+def isInstanceOfKnownType (ty : LMonoTy) (T : TEnv Identifier) : Bool :=
+  LMonoTy.knownInstance ty T.knownTypes
 
 /--
 Instantiate `ty`, with resolution of type aliases to type definitions and checks
 for registered types.
 -/
 def LTy.instantiateWithCheck (ty : LTy) (T : (TEnv Identifier)) : Except Format (LMonoTy × (TEnv Identifier)) := do
-  let (mty, T) := match ty.aliasInst T with
+  let (mty, T) := match ty.resolveAliases T with
                   | (some ty', T) => (ty', T)
                   | (none, T) => ty.instantiate T
   if isInstanceOfKnownType mty T
@@ -532,11 +582,9 @@ open LTy.Syntax
 /-- info: false -/
 #guard_msgs in
 #eval isInstanceOfKnownType mty[myTy (myTy)]
-                            { @TEnv.default String with knownTypes := [t[∀a. myTy %a], t[int]] }
-
-/-- info: true -/
-#guard_msgs in
-#eval isInstanceOfKnownType mty[%a → %a] (@TEnv.default String)
+                            { @TEnv.default String with
+                                knownTypes := [LTy.toKnownType! t[∀a. myTy %a],
+                                               LTy.toKnownType! t[int]] }
 
 /-- info: false -/
 #guard_msgs in
@@ -544,7 +592,7 @@ open LTy.Syntax
 
 /--
 info: error: Type (arrow int Foo) is not an instance of a previously registered type!
-Known Types: [∀[a, b]. (arrow a b), bool, int, string]
+Known Types: [∀[0, 1]. (arrow 0 1), bool, int, string]
 -/
 #guard_msgs in
 #eval do let ans ← t[int → Foo].instantiateWithCheck (@TEnv.default TyIdentifier)
@@ -631,9 +679,9 @@ info: ok: (x : $__ty0) (y : int) (z : $__ty0)
 open LTy.Syntax in
 #eval do let ans ← (LMonoTySignature.instantiate
                     { @TEnv.default TyIdentifier with context :=
-                                          { aliases := [{ args := ["a", "b"],
-                                                          lhs := mty[myInt %a %b],
-                                                          rhs := mty[int]}] }}
+                                          { aliases := [{ typeArgs := ["a", "b"],
+                                                          name := "myInt",
+                                                          type := mty[int]}] }}
                     ["a", "b"]
                     [("x", mty[%a]), ("y", mty[myInt %a %b]), ("z", mty[%a])])
          return Signature.format ans.fst
@@ -674,6 +722,41 @@ def TEnv.addInOldestContext (fvs : (IdentTs Identifier)) (T : (TEnv Identifier))
   let tys := monotys.map (fun mty => LTy.forAll [] mty)
   let types := T.context.types.addInOldest fvs.idents tys
   { T with context := { T.context with types := types } }
+
+/--
+Add a well-formed `alias` to the context, where the type definition is first
+de-aliased.
+-/
+def TEnv.addTypeAlias (alias : TypeAlias) (T : TEnv Identifier) : Except Format (TEnv Identifier) := do
+  let alias_lty := alias.toAliasLTy
+  if !alias.typeArgs.Nodup then
+    .error f!"[TEnv.addTypeAlias] Duplicates found in the type arguments!\n\
+               Name: {alias.name}\n\
+               Type Arguments: {alias.typeArgs}\n\
+               Type Definition: {alias.type}"
+  else if !((alias.type.freeVars ⊆ alias.typeArgs) &&
+            (alias_lty.freeVars ⊆ alias.typeArgs)) then
+    .error f!"[TEnv.addTypeAlias] Type definition contains free type arguments!\n\
+              Name: {alias.name}\n\
+              Type Arguments: {alias.typeArgs}\n\
+              Type Definition: {alias.type}"
+  else
+    let (mtys, T) := LMonoTys.instantiate alias.typeArgs [alias_lty.toMonoTypeUnsafe, alias.type] T
+    match mtys with
+    | [lhs, rhs] =>
+      let newTyArgs := lhs.freeVars
+      -- We expect `alias.type` to be a known, legal type, hence the use of
+      -- `instantiateWithCheck` below. Note that we only store type
+      -- declarations -- not synonyms -- as values in the alias table;
+      -- i.e., we don't store a type alias mapped to another type alias.
+      let (rhsmty, _) ← (LTy.forAll [] rhs).instantiateWithCheck T
+      let new_aliases := { typeArgs := newTyArgs,
+                           name := alias.name,
+                           type := rhsmty } :: T.context.aliases
+      let context := { T.context with aliases := new_aliases }
+      .ok { T with context := context }
+    | _ => .error f!"[TEnv.addTypeAlias] Implementation error! \n\
+                      {alias}"
 
 ---------------------------------------------------------------------
 
