Strata/Languages/Boogie/StatementType.lean
@@ -54,9 +54,7 @@ def typeCheckCmd (T : (TEnv BoogieIdent)) (P : Program) (c : Command) :
            let _ ← T.freeVarChecks args
            let (ret_sig, T) ← LMonoTySignature.instantiate T proc.header.typeArgs proc.header.outputs
            let ret_mtys := LMonoTys.subst T.state.substInfo.subst ret_sig.values
-           let constraints := lhs_tys.zip ret_mtys
-           let S ← Constraints.unify constraints T.state.substInfo
-           let T := T.updateSubst S
+           let ret_lhs_constraints := lhs_tys.zip ret_mtys
            -- Infer the types of the actuals and unify with the types of the
            -- procedure's formals.
            let (argsa, T) ← Lambda.LExprT.fromLExprs T args
@@ -64,8 +62,8 @@ def typeCheckCmd (T : (TEnv BoogieIdent)) (P : Program) (c : Command) :
            let args' := argsa.map $ LExprT.toLExpr
            let (inp_sig, T) ← LMonoTySignature.instantiate T proc.header.typeArgs proc.header.inputs
            let inp_mtys := LMonoTys.subst T.state.substInfo.subst inp_sig.values
-           let constraints := args_tys.zip inp_mtys
-           let S ← Constraints.unify constraints T.state.substInfo
+           let lhs_inp_constraints := (args_tys.zip inp_mtys)
+           let S ← Constraints.unify (lhs_inp_constraints ++ ret_lhs_constraints) T.state.substInfo
            let T := T.updateSubst S
            let s' := .call lhs pname args' md
            .ok (s', T)
@@ -73,82 +71,85 @@ def typeCheckCmd (T : (TEnv BoogieIdent)) (P : Program) (c : Command) :
 
 def typeCheckAux (T : (TEnv BoogieIdent)) (P : Program) (op : Option Procedure) (ss : List Statement) :
   Except Format (List Statement × (TEnv BoogieIdent)) :=
-  match ss with
-  | [] => .ok (ss, T)
-  | s :: srest => do
-    let (s', T) ←
-      match s with
-      | .cmd cmd => do
-        let (c', T) ← typeCheckCmd T P cmd
-        .ok (.cmd c', T)
+  go T ss []
+where
+  go (T : TEnv BoogieIdent) (ss : List Statement) (acc : List Statement) :
+    Except Format (List Statement × (TEnv BoogieIdent)) :=
+    match ss with
+    | [] => .ok (acc.reverse, T)
+    | s :: srest => do
+      let (s', T) ←
+        match s with
+        | .cmd cmd => do
+          let (c', T) ← typeCheckCmd T P cmd
+          .ok (.cmd c', T)
 
-      | .block label blk md => do
-        let T := T.pushEmptyContext
-        let (ss', T) ← typeCheckAux T P op blk.ss
-        let s' := .block label ⟨ss'⟩ md
-        .ok (s', T.popContext)
+        | .block label blk md => do
+          let T := T.pushEmptyContext
+          let (ss', T) ← go T blk.ss []
+          let s' := .block label ⟨ss'⟩ md
+          .ok (s', T.popContext)
 
-      | .ite cond thenb elseb md => do
-        let _ ← T.freeVarCheck cond f!"[{s}]"
-        let (conda, T) ← LExprT.fromLExpr T cond
-        let condty := conda.toLMonoTy
-        match condty with
-        | .tcons "bool" [] =>
-          let (tb, T) ← typeCheckAux T P op [(.block "$$_then" thenb #[])]
-          let (eb, T) ← typeCheckAux T P op [(.block "$$_else" elseb #[])]
-          let s' := .ite conda.toLExpr ⟨tb⟩ ⟨eb⟩ md
-          .ok (s', T)
-        | _ => .error f!"[{s}]: If's condition {cond} is not of type `bool`!"
-
-      | .loop guard measure invariant body md => do
-        let _ ← T.freeVarCheck guard f!"[{s}]"
-        let (conda, T) ← LExprT.fromLExpr T guard
-        let condty := conda.toLMonoTy
-        let (mty, T) ← match measure with
-        | .some m => do
-          let _ ← T.freeVarCheck m f!"[{s}]"
-          let (ma, T) ← LExprT.fromLExpr T m
-          .ok ((some ma.toLMonoTy), T)
-        | _ => .ok (none, T)
-        let (ity, T) ← match invariant with
-        | .some i => do
-          let _ ← T.freeVarCheck i f!"[{s}]"
-          let (ia, T) ← LExprT.fromLExpr T i
-          .ok ((some ia.toLMonoTy), T)
-        | _ => .ok (none, T)
-        match (condty, mty, ity) with
-        | (.tcons "bool" [], none, none)
-        | (.tcons "bool" [], some (.tcons "int" []), none)
-        | (.tcons "bool" [], none, some (.tcons "bool" []))
-        | (.tcons "bool" [], some (.tcons "int" []), some (.tcons "bool" [])) =>
-          let (tb, T) ← typeCheckAux T P op [(.block "$$_loop_body" body #[])]
-          let s' := .loop conda.toLExpr measure invariant ⟨tb⟩ md
-          .ok (s', T)
-        | _ =>
+        | .ite cond thenb elseb md => do
+          let _ ← T.freeVarCheck cond f!"[{s}]"
+          let (conda, T) ← LExprT.fromLExpr T cond
+          let condty := conda.toLMonoTy
           match condty with
           | .tcons "bool" [] =>
-            match mty with
-            | none | .some (.tcons "int" []) =>
-              match ity with
-              | none | .some (.tcons "bool" []) => panic! "Internal error. condty, mty or ity must be unexpected."
-              | _ => .error f!"[{s}]: Loop's invariant {invariant} is not of type `bool`!"
-            | _ => .error f!"[{s}]: Loop's measure {measure} is not of type `int`!"
-          | _ =>  .error f!"[{s}]: Loop's guard {guard} is not of type `bool`!"
+            let (tb, T) ← go T [(.block "$$_then" thenb #[])] []
+            let (eb, T) ← go T [(.block "$$_else" elseb #[])] []
+            let s' := .ite conda.toLExpr ⟨tb⟩ ⟨eb⟩ md
+            .ok (s', T)
+          | _ => .error f!"[{s}]: If's condition {cond} is not of type `bool`!"
 
-      | .goto label _ =>
-        match op with
-        | .some p =>
-          if Stmts.hasLabelInside label p.body then
-            .ok (s, T)
-          else
-            .error f!"Label {label} does not exist in the body of {p.header.name}"
-        | .none => .error f!"{s} occurs outside a procedure."
+        | .loop guard measure invariant body md => do
+          let _ ← T.freeVarCheck guard f!"[{s}]"
+          let (conda, T) ← LExprT.fromLExpr T guard
+          let condty := conda.toLMonoTy
+          let (mty, T) ← match measure with
+          | .some m => do
+            let _ ← T.freeVarCheck m f!"[{s}]"
+            let (ma, T) ← LExprT.fromLExpr T m
+            .ok ((some ma.toLMonoTy), T)
+          | _ => .ok (none, T)
+          let (ity, T) ← match invariant with
+          | .some i => do
+            let _ ← T.freeVarCheck i f!"[{s}]"
+            let (ia, T) ← LExprT.fromLExpr T i
+            .ok ((some ia.toLMonoTy), T)
+          | _ => .ok (none, T)
+          match (condty, mty, ity) with
+          | (.tcons "bool" [], none, none)
+          | (.tcons "bool" [], some (.tcons "int" []), none)
+          | (.tcons "bool" [], none, some (.tcons "bool" []))
+          | (.tcons "bool" [], some (.tcons "int" []), some (.tcons "bool" [])) =>
+            let (tb, T) ← go T [(.block "$$_loop_body" body #[])] []
+            let s' := .loop conda.toLExpr measure invariant ⟨tb⟩ md
+            .ok (s', T)
+          | _ =>
+            match condty with
+            | .tcons "bool" [] =>
+              match mty with
+              | none | .some (.tcons "int" []) =>
+                match ity with
+                | none | .some (.tcons "bool" []) => panic! "Internal error. condty, mty or ity must be unexpected."
+                | _ => .error f!"[{s}]: Loop's invariant {invariant} is not of type `bool`!"
+              | _ => .error f!"[{s}]: Loop's measure {measure} is not of type `int`!"
+            | _ =>  .error f!"[{s}]: Loop's guard {guard} is not of type `bool`!"
 
-    let (ss', T) ← typeCheckAux T P op srest
-    .ok (s' :: ss', T)
-  termination_by Stmts.sizeOf ss
-  decreasing_by
-  all_goals simp_wf <;> omega
+        | .goto label _ =>
+          match op with
+          | .some p =>
+            if Stmts.hasLabelInside label p.body then
+              .ok (s, T)
+            else
+              .error f!"Label {label} does not exist in the body of {p.header.name}"
+          | .none => .error f!"{s} occurs outside a procedure."
+
+      go T srest (s' :: acc)
+    termination_by Stmts.sizeOf ss
+    decreasing_by
+    all_goals simp_wf <;> omega
 
 /--
 Apply type substitution `S` to a command.
@@ -177,24 +178,23 @@ private def substOptionExpr (S : Subst) (oe : Option Expression.Expr) : Option E
 Apply type substitution `S` to a statement.
 -/
 def Statement.subst (S : Subst) (s : Statement) : Statement :=
-
   match s with
   | .cmd cmd => .cmd (Command.subst S cmd)
   | .block label b md =>
-    .block label ⟨go S b.ss⟩ md
+    .block label ⟨go S b.ss []⟩ md
   | .ite cond thenb elseb md =>
-    .ite (cond.applySubst S) ⟨go S thenb.ss⟩ ⟨go S elseb.ss⟩ md
+    .ite (cond.applySubst S) ⟨go S thenb.ss []⟩ ⟨go S elseb.ss []⟩ md
   | .loop guard m i body md =>
-    .loop (guard.applySubst S) (substOptionExpr S m) (substOptionExpr S i) ⟨go S body.ss⟩ md
+    .loop (guard.applySubst S) (substOptionExpr S m) (substOptionExpr S i) ⟨go S body.ss []⟩ md
   | .goto _ _ => s
   termination_by (Stmt.sizeOf s)
   decreasing_by
     all_goals simp_wf <;> omega
   where
-    go S ss : List Statement :=
+    go S ss acc : List Statement :=
     match ss with
-    | [] => []
-    | s :: srest => Statement.subst S s :: go S srest
+    | [] => acc.reverse
+    | s :: srest => go S srest ((Statement.subst S s) :: acc)
     termination_by (Stmts.sizeOf ss)
     decreasing_by
       all_goals simp_wf <;> omega
@@ -211,7 +211,7 @@ def typeCheck (T : Expression.TyEnv) (P : Program) (op : Option Procedure) (ss :
   let (ss', T) ← typeCheckAux T P op ss
   let context := TContext.subst T.context T.state.substInfo.subst
   let T := { T with context := context }
-  let ss' := Statement.subst.go T.state.substInfo.subst ss'
+  let ss' := Statement.subst.go T.state.substInfo.subst ss' []
   .ok (ss', T)
 
 ---------------------------------------------------------------------
